messageInvariantPrototypes/flexPaxos/decentralizedMonotonicTemplated/monotonicityInvariants.dfy
@@ -1,0 +1,99 @@
+include "spec.dfy"
+
+module MonotonicityInvariants {
+import opened Types
+import opened UtilitiesLibrary
+import opened MonotonicityLibrary
+import opened DistributedSystem
+
+/***************************************************************************************
+*                               Monotonicity Invariants                                *
+***************************************************************************************/
+
+ghost predicate LeaderReceivedPromisesAndValueMonotonic(c: Constants, v: Variables)
+  requires v.WF(c)
+{
+  forall i, j, ldr |
+    && v.ValidHistoryIdx(i)
+    && v.ValidHistoryIdx(j)
+    && i <= j
+    && c.ValidLeaderIdx(ldr)
+  :: 
+    v.History(j).leaders[ldr].receivedPromisesAndValue.SatisfiesMonotonic(v.History(i).leaders[ldr].receivedPromisesAndValue)
+}
+
+ghost predicate LeaderHighestHeardMonotonic(c: Constants, v: Variables)
+  requires v.WF(c)
+{
+  forall i, j, ldr |
+    && v.ValidHistoryIdx(i)
+    && v.ValidHistoryIdx(j)
+    && i <= j
+    && c.ValidLeaderIdx(ldr)
+  :: 
+    v.History(j).leaders[ldr].highestHeardBallot.SatisfiesMonotonic(v.History(i).leaders[ldr].highestHeardBallot)
+}
+
+ghost predicate AcceptorAcceptedMonotonic(c: Constants, v: Variables)
+  requires v.WF(c)
+{
+  forall i, j, acc | 
+    && v.ValidHistoryIdx(i)
+    && v.ValidHistoryIdx(j)
+    && c.ValidAcceptorIdx(acc)
+    && i <= j
+  ::
+    v.History(j).acceptors[acc].acceptedVB.SatisfiesMonotonic(v.History(i).acceptors[acc].acceptedVB)
+}
+
+ghost predicate AcceptorPromisedMonotonic(c: Constants, v: Variables)
+  requires v.WF(c)
+{
+  forall i, j, acc | 
+    && v.ValidHistoryIdx(i)
+    && v.ValidHistoryIdx(j)
+    && c.ValidAcceptorIdx(acc)
+    && i <= j
+  ::
+    v.History(j).acceptors[acc].promised.SatisfiesMonotonic(v.History(i).acceptors[acc].promised)
+}
+
+ghost predicate LearnerReceivedAcceptsMonotonic(c: Constants, v: Variables)
+  requires v.WF(c)
+{
+  forall i, j, lnr | 
+    && v.ValidHistoryIdx(i)
+    && v.ValidHistoryIdx(j)
+    && c.ValidLearnerIdx(lnr)
+    && i <= j
+  ::
+    v.History(j).learners[lnr].receivedAccepts.SatisfiesMonotonic(v.History(i).learners[lnr].receivedAccepts)
+}
+
+ghost predicate MonotonicityInv(c: Constants, v: Variables) 
+{
+  && v.WF(c)
+  && LeaderHighestHeardMonotonic(c, v)
+  && LeaderReceivedPromisesAndValueMonotonic(c, v)
+  && AcceptorAcceptedMonotonic(c, v)
+  && AcceptorPromisedMonotonic(c, v)
+  && LearnerReceivedAcceptsMonotonic(c, v)
+}
+
+// Base obligation
+lemma InitImpliesMonotonicityInv(c: Constants, v: Variables)
+  requires Init(c, v)
+  ensures MonotonicityInv(c, v)
+{}
+
+// Inductive obligation
+lemma MonotonicityInvInductive(c: Constants, v: Variables, v': Variables)
+  requires MonotonicityInv(c, v)
+  requires Next(c, v, v')
+  ensures MonotonicityInv(c, v')
+{
+  VariableNextProperties(c, v, v');
+}
+
+} // end module MonotonicityInvariants
+
